core(imp): Break down for optim into two steps
Signed-off-by: Jerome Simeon <jeromesimeon@me.com>

compiler/core/Imp/Optim/ImpEJsonRewrite.v
@@ -35,46 +35,173 @@ Section ImpEJsonRewrite.
   Context {foreign_ejson_runtime_op : Set}.
   Context {fejruntime:foreign_ejson_runtime foreign_ejson_runtime_op}.
 
-  Lemma imp_ejson_stmt_eval_env_simpl h stmt l1 x v l2:
-    ~ In x (domain l2) ->
-    imp_ejson_stmt_eval h stmt (l1 ++ (x, v) :: l2) = imp_ejson_stmt_eval h stmt (l1 ++ l2).
-  Proof.
-    admit.
-  Admitted.
+  Section ForLetRewrite.
+
+    (* Rewriting functional for into imperative for loop is now isolated *)
+    Definition imp_ejson_stmt_for_let_rewrite (stmt: @imp_ejson_stmt foreign_ejson_model foreign_ejson_runtime_op): imp_ejson_stmt :=
+      match stmt with
+      | ImpStmtFor v e s =>
+        (**
+              for(v in e) do s done
+              (src) fresh in v::s
+              ============================
+              { let src = e;
+                for(v in src) do s done }
+         *)
+        let avoid := v :: imp_ejson_stmt_free_vars s in
+        let src_id := fresh_var "src" avoid in
+        let src := ImpExprVar src_id in
+        ImpStmtBlock
+          [ (src_id, Some e) ]
+          [ ImpStmtFor v src s ]
+      | _ => stmt
+      end.
+
+  End ForLetRewrite.
+
+  Section CorrectnessForLetRewrite.
+
+    Lemma lookup_first_var A (i0 : A) (v:var) σ :
+      lookup EquivDec.equiv_dec ((v, i0) :: σ) v = Some i0.
+    Proof.
+      simpl.
+      destruct (EquivDec.equiv_dec v v); try congruence.
+    Qed.
+
+    Lemma test1 h stmt v j σ σ':
+      imp_ejson_stmt_eval h stmt
+        ((fresh_var "src" (v :: imp_ejson_stmt_free_vars stmt), j) :: σ) = Some ((fresh_var "src" (v :: imp_ejson_stmt_free_vars stmt), j) :: σ') ->
+      imp_ejson_stmt_eval h stmt σ = Some σ'.
+    Proof.
+      imp_stmt_cases (destruct stmt) Case; simpl; intros.
+      - admit.
+      - admit.
+      - admit.
+      - admit.
+      - admit.
+    Admitted.
+
+    Lemma test2 h stmt x1 v j σ:
+      imp_ejson_stmt_eval h stmt
+        (x1 :: (fresh_var "src" (v :: imp_ejson_stmt_free_vars stmt), Some j) :: σ) = None <->
+      imp_ejson_stmt_eval h stmt (x1 :: σ) = None.
+    Proof.
+      admit.
+    Admitted.
+
+    Lemma test3 h stmt v l σ σ' i0 :
+      (fix for_fun
+           (dl : list imp_ejson_model) (σ₁ : list (var * option imp_ejson_model)) {struct dl} :
+         option (list (var * option imp_ejson_model)) :=
+         match dl with
+         | [] => Some σ₁
+         | d :: dl' =>
+           match imp_ejson_stmt_eval h stmt ((v, Some d) :: σ₁) with
+           | Some (_ :: σ₂) => for_fun dl' σ₂
+           | _ => None
+           end
+         end) l σ = Some σ' ->
+      (fix for_fun
+       (dl : list imp_ejson_model) (σ₁ : list (var * option imp_ejson_model)) {struct dl} :
+         option (list (var * option imp_ejson_model)) :=
+       match dl with
+       | [] => Some σ₁
+       | d :: dl' =>
+           match imp_ejson_stmt_eval h stmt ((v, Some d) :: σ₁) with
+           | Some (_ :: σ₂) => for_fun dl' σ₂
+           | _ => None
+           end
+       end) l ((fresh_var "src" (v :: imp_ejson_stmt_free_vars stmt), Some i0) :: σ) = Some ((fresh_var "src" (v :: imp_ejson_stmt_free_vars stmt), Some i0) :: σ').
+    Proof.
+      admit.
+    Admitted.
+
+    Lemma test4 h stmt v l σ i0 :
+      (fix for_fun
+           (dl : list imp_ejson_model) (σ₁ : list (var * option imp_ejson_model)) {struct dl} :
+         option (list (var * option imp_ejson_model)) :=
+         match dl with
+         | [] => Some σ₁
+         | d :: dl' =>
+           match imp_ejson_stmt_eval h stmt ((v, Some d) :: σ₁) with
+           | Some (_ :: σ₂) => for_fun dl' σ₂
+           | _ => None
+           end
+         end) l σ = None ->
+      (fix for_fun
+       (dl : list imp_ejson_model) (σ₁ : list (var * option imp_ejson_model)) {struct dl} :
+         option (list (var * option imp_ejson_model)) :=
+       match dl with
+       | [] => Some σ₁
+       | d :: dl' =>
+           match imp_ejson_stmt_eval h stmt ((v, Some d) :: σ₁) with
+           | Some (_ :: σ₂) => for_fun dl' σ₂
+           | _ => None
+           end
+       end) l ((fresh_var "src" (v :: imp_ejson_stmt_free_vars stmt), Some i0) :: σ) = None.
+    Proof.
+      admit.
+    Admitted.
+
+    Lemma test5 h stmt v i0 i1 σ:
+      imp_ejson_stmt_eval h stmt ((v, Some i1) :: σ) = None ->
+      imp_ejson_stmt_eval h stmt
+                          ((v, Some i1) :: (fresh_var "src" (v :: imp_ejson_stmt_free_vars stmt), Some i0) :: σ) = None.
+    Proof.
+      admit.
+    Admitted.
+    
+    Lemma imp_ejson_stmt_for_let_rewrite_correct h (σ : pd_jbindings) (stmt:imp_ejson_stmt) :
+        imp_ejson_stmt_eval h stmt σ =
+        imp_ejson_stmt_eval h (imp_ejson_stmt_for_let_rewrite stmt) σ.
+    Proof.
+      destruct stmt; try reflexivity.
+      simpl.
+      unfold ImpEval.imp_decls_eval; unfold olift; simpl.
+      generalize (@ImpEval.imp_expr_eval (@imp_ejson_model foreign_ejson_model)
+        (@imp_ejson_constant foreign_ejson_model) imp_ejson_op
+        (@imp_ejson_runtime_op foreign_ejson_runtime_op)
+        (@imp_ejson_model_normalize foreign_ejson_model)
+        (@imp_ejson_runtime_eval foreign_ejson_model fejson foreign_ejson_runtime_op fejruntime h)
+        (@imp_ejson_op_eval foreign_ejson_model) σ i); intros; clear i.
+      destruct o; try reflexivity.
+      rewrite lookup_first_var.
+      destruct (imp_ejson_model_to_list i); try reflexivity.
+      admit.
+    Admitted.
+
+  End CorrectnessForLetRewrite.
 
   Section ForRewrite.
 
     (* Rewriting functional for into imperative for loop is now isolated *)
     Definition imp_ejson_stmt_for_rewrite (stmt: @imp_ejson_stmt foreign_ejson_model foreign_ejson_runtime_op): imp_ejson_stmt :=
       match stmt with
-      | ImpStmtFor v e s =>
+      | ImpStmtFor v (ImpExprVar src_id) s =>
         (**
-              for(v in e) do s done
-              (i,src) fresh in v::s
+              for(v in vsrc) do s done // vsrc is variable
+              vi fresh in s
               ============================
-              { let src = e;
-                for(i = 0 to length(e)-1) do
-                  { let v = src[i];
-                    s }
-                done }
+              for(i = 0 to length(vsrc)-1) do
+                { let v = vsrc[i];
+                  s }
+              done
          *)
-        let avoid := v :: imp_ejson_stmt_free_vars stmt in
+        let avoid := imp_ejson_stmt_free_vars stmt in
         let i_id := fresh_var "i" avoid in
         let avoid := i_id :: avoid in
-        let src_id := fresh_var "src" avoid in
-        let src := ImpExprVar src_id in
         let i := ImpExprVar i_id in
-        ImpStmtBlock
-          [ (src_id, Some e) ]
-          [ ImpStmtForRange
-              i_id
-              (ImpExprConst (cejbigint 0))
-              (* XXX Use src.length - 1, consistent with semantic of 'for i1 to i2 do ... done' loop *)
-              (ImpExprRuntimeCall EJsonRuntimeNatMinus
-                                  [ ImpExprRuntimeCall EJsonRuntimeArrayLength [ src ] ; ImpExprConst (cejbigint 1) ])
-              (ImpStmtBlock
-                 [ (v, Some (ImpExprRuntimeCall EJsonRuntimeArrayAccess [ src; i ])) ]
-                 [ s ]) ]
+        ImpStmtForRange
+          i_id
+          (ImpExprConst (cejbigint 0))
+          (* XXX Use src.length - 1, consistent with semantic of 'for i1 to i2 do ... done' loop *)
+          (ImpExprRuntimeCall
+             EJsonRuntimeNatMinus [
+               ImpExprRuntimeCall EJsonRuntimeArrayLength [ (ImpExprVar src_id) ]; ImpExprConst (cejbigint 1)
+          ])
+          (ImpStmtBlock
+             [ (v, Some (ImpExprRuntimeCall EJsonRuntimeArrayAccess [ (ImpExprVar src_id); i ])) ]
+             [ s ])
       | _ => stmt
       end.
   End ForRewrite.
@@ -109,357 +236,29 @@ Section ImpEJsonRewrite.
     Definition list_tail_n_nat {A} n (l: list A) :=
       List.rev (list_n_nat n (List.rev l)).
 
-    (*
-    Lemma for_corr_aux
-      (l_init : list ejson)
-      (j: nat)
-      (v : var)
-      (e : imp_expr)
-      (stmt : imp_stmt)
-      (h : BrandRelation.brand_relation_t)
-      (l : list ejson)
-      (σ : pd_jbindings) :
-      let i := fresh_var "i"
-                         (v :: imp_ejson_expr_free_vars e ++
-                            remove string_eqdec v (imp_ejson_stmt_free_vars stmt))
-      in
-      let src := fresh_var "src"
-                           (i :: v :: imp_ejson_expr_free_vars e ++
-                              remove string_eqdec v (imp_ejson_stmt_free_vars stmt))
-      in
-      (lookup string_eqdec σ src = Some (Some (ejarray l_init))) ->
-      (list_tail_n_nat (List.length l) l_init = l) ->
-      (j + Datatypes.length l = List.length l_init) ->
-      (fix for_fun (dl : list imp_ejson_model) (σ₁ : list (var * option imp_ejson_model)) {struct dl} :
-         option (list (var * option imp_ejson_model)) :=
-         match dl with
-         | [] => Some σ₁
-         | d :: dl' =>
-           match imp_ejson_stmt_eval h stmt ((v, Some d) :: σ₁) with
-           | Some (_ :: σ₂) => for_fun dl' σ₂
-           | _ => None
-           end
-         end) l σ =
-       match
-         (fix for_range (n : nat) (n1 : BinNums.Z) (σ₁ : list (var * option imp_ejson_model)) {struct n} :
-            option (list (var * option imp_ejson_model)) :=
-            match n with
-            | 0 => Some σ₁
-            | S n' =>
-                match
-                  match
-                    match
-                      match
-                        olift (imp_ejson_runtime_eval h EJsonRuntimeArrayAccess)
-                          match
-                            olift (fun x : option imp_ejson_model => x)
-                              ((fix
-                                lookup (l0 : list (string * option imp_ejson_model)) (a : string) {struct l0} :
-                                  option (option imp_ejson_model) :=
-                                  match l0 with
-                                  | [] => None
-                                  | (f', v') :: os => if EquivDec.equiv_dec a f' then Some v' else lookup os a
-                                  end) σ₁
-                                 src)
-                          with
-                          | Some x' => Some [x'; imp_ejson_Z_to_data n1]
-                          | None => None
-                          end
-                      with
-                      | Some d =>
-                          Some
-                            ((v, Some d)
-                             :: (i, Some (imp_ejson_Z_to_data n1))
-                             :: σ₁)
-                      | None => None
-                      end
-                    with
-                    | Some x' => imp_ejson_stmt_eval h stmt x'
-                    | None => None
-                    end
-                  with
-                  | Some (_ :: σ') => Some σ'
-                  | _ => None
-                  end
-                with
-                | Some (_ :: σ₂) => for_range n' (BinInt.Z.add n1 1) σ₂
-                | _ => None
-                end
-            end) (j + Datatypes.length l) (BinInt.Z_of_nat j)
-           ((src, Some (ejarray l)) :: σ)
-       with
-       | Some (_ :: σ') => Some σ'
-       | _ => None
-       end.
-    Proof.
-      admit.
-    Admitted.
-     *)
-
-    (* Lemma for_range_ind h src i j n s σ : *)
-    (*   let for_range_stmt := ImpStmtForRange i j n s in *)
-    (*   j <= n -> *)
-    (*   imp_ejson_expr_eval h (ImpExprVar src) σ = Some l_init -> *)
-      
-
-
-    Lemma for_corr v e stmt :
-      forall h σ,
-      let for_stmt := ImpStmtFor v e stmt in
-      let for_range_stmt :=
-        let avoid := v :: imp_ejson_stmt_free_vars (ImpStmtFor v e stmt) in
-        let i_id := fresh_var "i" avoid in
-        let avoid := i_id :: avoid in
-        let src_id := fresh_var "src" avoid in
-        let src := ImpExprVar src_id in
-        let i := ImpExprVar i_id in
-        ImpStmtBlock
-          [ (src_id, Some e) ]
-          [ ImpStmtForRange
-              i_id
-              (ImpExprConst (cejbigint 0))
-              (* XXX Use src.length - 1, consistent with semantic of 'for i1 to i2 do ... done' loop *)
-              (ImpExprRuntimeCall EJsonRuntimeNatMinus
-                                  [ ImpExprRuntimeCall EJsonRuntimeArrayLength [ src ] ; ImpExprConst (cejbigint 1) ])
-              (ImpStmtBlock
-                 [ (v, Some (ImpExprRuntimeCall EJsonRuntimeArrayAccess [ src; i ])) ]
-                 [ stmt ]) ]
-      in
-      imp_ejson_stmt_eval h for_stmt σ =
-      imp_ejson_stmt_eval h for_range_stmt σ.
-    Proof.
-      simpl.
-      intros.
-      unfold ImpEval.imp_decls_eval.
-      unfold olift.
-      simpl.
-      match_destr.
-      unfold lookup.
-      case (EquivDec.equiv_dec
-              (fresh_var "src"
-                 (fresh_var "i"
-                    (v
-                     :: ImpVars.imp_expr_free_vars e ++
-                        remove string_eqdec v (imp_ejson_stmt_free_vars stmt))
-                  :: v
-                     :: ImpVars.imp_expr_free_vars e ++
-                        remove string_eqdec v (imp_ejson_stmt_free_vars stmt)))
-              (fresh_var "src"
-                 (fresh_var "i"
-                    (v
-                     :: ImpVars.imp_expr_free_vars e ++
-                        remove string_eqdec v (imp_ejson_stmt_free_vars stmt))
-                  :: v
-                     :: ImpVars.imp_expr_free_vars e ++
-                        remove string_eqdec v (imp_ejson_stmt_free_vars stmt))));
-        [ intro Eq; clear Eq | congruence ].
-      case (EquivDec.equiv_dec
-               (fresh_var "i"
-                  (v
-                   :: ImpVars.imp_expr_free_vars e ++
-                      remove string_eqdec v (imp_ejson_stmt_free_vars stmt)))
-               (fresh_var "i"
-                  (v
-                   :: ImpVars.imp_expr_free_vars e ++
-                      remove string_eqdec v (imp_ejson_stmt_free_vars stmt))));
-        try congruence; intro Eq; clear Eq.
-      unfold imp_ejson_model_to_list.
-      case i; simpl; try reflexivity.
-      intros l.
-      rewrite number_iterations.
-      generalize σ; clear σ.
-
-
-      induction l; [ simpl; reflexivity | ].
-      intros.
-      simpl.
-
-        unfold olift.
-        case (EquivDec.equiv_dec
-                (fresh_var "src"
-                   (fresh_var "i"
-                      (v
-                       :: ImpVars.imp_expr_free_vars e ++
-                          remove string_eqdec v (imp_ejson_stmt_free_vars stmt))
-                    :: v
-                       :: ImpVars.imp_expr_free_vars e ++
-                          remove string_eqdec v (imp_ejson_stmt_free_vars stmt)))
-                (fresh_var "src"
-                   (fresh_var "i"
-                      (v
-                       :: ImpVars.imp_expr_free_vars e ++
-                          remove string_eqdec v (imp_ejson_stmt_free_vars stmt))
-                    :: v
-                       :: ImpVars.imp_expr_free_vars e ++
-                          remove string_eqdec v (imp_ejson_stmt_free_vars stmt))));
-          [ intro Eq; clear Eq | congruence].
-        simpl.
-        rewrite (imp_ejson_stmt_eval_env_simpl _ _
-                   ((v, Some a)
-                    :: (fresh_var "i"
-                          (v
-                           :: ImpVars.imp_expr_free_vars e ++ remove string_eqdec v (imp_ejson_stmt_free_vars stmt)),
-                       Some (imp_ejson_Z_to_data 0)) :: [])
-                   (fresh_var "src"
-                     (fresh_var "i"
-                        (v
-                         :: ImpVars.imp_expr_free_vars e ++
-                            remove string_eqdec v (imp_ejson_stmt_free_vars stmt))
-                      :: v
-                         :: ImpVars.imp_expr_free_vars e ++
-                            remove string_eqdec v (imp_ejson_stmt_free_vars stmt)))
-                   (Some (ejarray (a :: l)))
-                   σ);
-          [ | admit ].
-        rewrite (imp_ejson_stmt_eval_env_simpl _ _
-                   ((v, Some a) :: [])
-                   (fresh_var "i"
-                     (v :: ImpVars.imp_expr_free_vars e ++ remove string_eqdec v (imp_ejson_stmt_free_vars stmt)))
-                   (Some (imp_ejson_Z_to_data 0))
-                   σ);
-          [ | admit ].
-        simpl.
-        unfold var.
-        unfold imp_ejson_model.
-        case (@imp_ejson_stmt_eval foreign_ejson_model fejson foreign_ejson_runtime_op fejruntime h stmt
-            (@cons (prod string (option (@ejson foreign_ejson_model)))
-               (@pair string (option (@ejson foreign_ejson_model)) v (@Some (@ejson foreign_ejson_model) a)) σ));
-          [ | simpl; reflexivity].
-        intros σ'.
-        clear i a σ.
-        match_destr.
-        rewrite IHl; clear IHl.
-        unfold olift.
-        simpl.
-        admit.
-    Admitted.
-
-    Lemma for_body h src i v n n' a stmt σ1:
-      (* match *)
-      (*   ImpEval.imp_decls_eval *)
-      (*     ((fresh_var "i" *)
-      (*         (fresh_var "src" *)
-      (*            ((ImpVars.imp_expr_free_vars e ++ *)
-      (*              remove string_eqdec v (imp_ejson_stmt_free_vars stmt)) ++ *)
-      (*             v :: imp_ejson_stmt_bound_vars stmt) *)
-      (*          :: (ImpVars.imp_expr_free_vars e ++ *)
-      (*              remove string_eqdec v (imp_ejson_stmt_free_vars stmt)) ++ *)
-      (*             v :: imp_ejson_stmt_bound_vars stmt), Some (imp_ejson_Z_to_data n1)) *)
-      (*      :: σ₁) *)
-      (*     [(v, *)
-      (*      Some *)
-      (*        (ImpExprOp EJsonRuntimeArrayAccess *)
-      (*           [ImpExprVar *)
-      (*              (fresh_var "src" *)
-      (*                 ((ImpVars.imp_expr_free_vars e ++ *)
-      (*                   remove string_eqdec v (imp_ejson_stmt_free_vars stmt)) ++ *)
-      (*                  v :: imp_ejson_stmt_bound_vars stmt)); *)
-      (*           ImpExprVar *)
-      (*             (fresh_var "i" *)
-      (*                (fresh_var "src" *)
-      (*                   ((ImpVars.imp_expr_free_vars e ++ *)
-      (*                     remove string_eqdec v (imp_ejson_stmt_free_vars stmt)) ++ *)
-      (*                    v :: imp_ejson_stmt_bound_vars stmt) *)
-      (*                 :: (ImpVars.imp_expr_free_vars e ++ *)
-      (*                     remove string_eqdec v (imp_ejson_stmt_free_vars stmt)) ++ *)
-      (*                    v :: imp_ejson_stmt_bound_vars stmt))]))] *)
-      (* with *)
-      (* | Some x'0 => imp_ejson_stmt_eval h (imp_ejson_stmt_for_rewrite stmt) x'0 *)
-      (* | None => None *)
-      (* end *)
-      imp_ejson_decls_eval h
-        ((i, Some (imp_ejson_Z_to_data n)) :: σ1)
-        [(v, Some (ImpExprRuntimeCall EJsonRuntimeArrayAccess [ImpExprVar src; ImpExprVar i]))]
-      =
-      Some ((v, a) :: (i, n') :: σ1)
-      ->
-      match
-        imp_ejson_decls_eval h
-          ((i, Some (imp_ejson_Z_to_data n)) :: σ1)
-          [(v, Some (ImpExprRuntimeCall EJsonRuntimeArrayAccess [ImpExprVar src; ImpExprVar i]))]
-      with
-      | Some σ2 => imp_ejson_stmt_eval h (imp_ejson_stmt_for_rewrite stmt) σ2
-      | None => None
-      end
-      =
-      imp_ejson_stmt_eval h stmt ((v, a) :: (i, n') :: σ1).
-    Proof.
-      admit.
-    Admitted.
-
     Lemma imp_ejson_stmt_for_rewrite_correct h (σ : pd_jbindings) (stmt:imp_ejson_stmt) :
         imp_ejson_stmt_eval h stmt σ =
         imp_ejson_stmt_eval h (imp_ejson_stmt_for_rewrite stmt) σ.
     Proof.
+      imp_stmt_cases (destruct stmt) Case; try reflexivity; intros.
+      simpl.
+      destruct i; try reflexivity; intros; simpl.
+      destruct (@olift (option (@imp_ejson_model foreign_ejson_model))
+        (@imp_ejson_model foreign_ejson_model)
+        (fun x : option (@imp_ejson_model foreign_ejson_model) => x)
+        (@lookup string (option (@imp_ejson_model foreign_ejson_model))
+           (@EquivDec.equiv_dec string (@eq string) (@RelationClasses.eq_equivalence string)
+              string_eqdec) σ v0)); try reflexivity.
+      simpl.
+      unfold imp_ejson_model_to_list.
+      case i; simpl; try reflexivity; intros l; clear i.
+      rewrite number_iterations.
       revert σ.
-      imp_stmt_cases (induction stmt) Case; try reflexivity; intros.
-      - Case "ImpStmtFor"%string.
-        simpl in *.
-        unfold ImpEval.imp_decls_eval.
-        unfold olift.
-        simpl.
-        match_destr.
-        unfold lookup.
-        (* case (EquivDec.equiv_dec (fresh_var "src" (v :: avoid)) (fresh_var "src" (v :: avoid))); *)
-        (*   try congruence; intro Eq; clear Eq. *)
-Set Printing Depth 100.
-        case (EquivDec.equiv_dec
-                (fresh_var "src"
-                   (fresh_var "i"
-                      (v
-                       :: ImpVars.imp_expr_free_vars e ++
-                          remove string_eqdec v (imp_ejson_stmt_free_vars stmt))
-                    :: v
-                       :: ImpVars.imp_expr_free_vars e ++
-                          remove string_eqdec v (imp_ejson_stmt_free_vars stmt)))
-                (fresh_var "src"
-                   (fresh_var "i"
-                      (v
-                       :: ImpVars.imp_expr_free_vars e ++
-                          remove string_eqdec v (imp_ejson_stmt_free_vars stmt))
-                    :: v
-                       :: ImpVars.imp_expr_free_vars e ++
-                          remove string_eqdec v (imp_ejson_stmt_free_vars stmt))));
-          [ intro Eq; clear Eq | congruence ].
-        case (EquivDec.equiv_dec
-                 (fresh_var "i"
-                    (v
-                     :: ImpVars.imp_expr_free_vars e ++
-                        remove string_eqdec v (imp_ejson_stmt_free_vars stmt)))
-                 (fresh_var "i"
-                    (v
-                     :: ImpVars.imp_expr_free_vars e ++
-                        remove string_eqdec v (imp_ejson_stmt_free_vars stmt))));
-          try congruence; intro Eq; clear Eq.
-        unfold imp_ejson_model_to_list.
-        case i; simpl; try reflexivity.
-        intros l.
-        rewrite number_iterations.
-        revert σ.
-        induction l; [ simpl; reflexivity | ].
-        intros.
-        simpl.
-        unfold olift.
-        case (EquivDec.equiv_dec
-                (fresh_var "src"
-                   (fresh_var "i"
-                      (v
-                       :: ImpVars.imp_expr_free_vars e ++
-                          remove string_eqdec v (imp_ejson_stmt_free_vars stmt))
-                    :: v
-                       :: ImpVars.imp_expr_free_vars e ++
-                          remove string_eqdec v (imp_ejson_stmt_free_vars stmt)))
-                (fresh_var "src"
-                   (fresh_var "i"
-                      (v
-                       :: ImpVars.imp_expr_free_vars e ++
-                          remove string_eqdec v (imp_ejson_stmt_free_vars stmt))
-                    :: v
-                       :: ImpVars.imp_expr_free_vars e ++
-                          remove string_eqdec v (imp_ejson_stmt_free_vars stmt))));
-          [ intro Eq; clear Eq | congruence].
-        simpl.
-        admit.
+      induction l; [ simpl; reflexivity | ].
+      intros.
+      simpl.
+      unfold olift.
+      admit.
     Admitted.
 
   End CorrectnessForRewrite.
